.

pure/Data.v
@@ -17,95 +17,23 @@ Module BinTree.
   | Dir_right : dir_t
   .
 
-  Definition dir_compare (d1 : dir_t) (d2 : dir_t) : comparison :=
-    match d1, d2 with
-    | Dir_left, Dir_left => Eq
-    | Dir_left, Dir_right => Lt
-    | Dir_right, Dir_left => Gt
-    | Dir_right, Dir_right => Eq
-    end
-  .
-
-  Global Program Instance dir_isPoset : isPoset dir_t :=
-    { leProp :=
-      fun d1 : dir_t =>
-      fun d2 : dir_t =>
-      dir_compare d1 d2 = Lt \/ dir_compare d1 d2 = Eq
-    ; Poset_requiresSetoid :=
-      {| eqProp := @eq dir_t; Setoid_requiresEquivalence := eq_equivalence |}
-    }
-  .
-
-  Next Obligation with eauto with *.
-    split.
-    - intros [ | ]...
-    - intros [ | ] [ | ] [ | ]...
-  Qed.
-
-  Next Obligation with discriminate || eauto with *.
-    intros d1 d2; split; cbn; unfold Basics.flip.
-    all: destruct d1 as [ | ]; destruct d2 as [ | ]...
-    all: intros [[ | ] [ | ]]...
-  Qed.
-
-  Lemma dir_compare_spec_LT :
-    forall lhs : dir_t,
-    forall rhs : dir_t, dir_compare lhs rhs = Lt ->
-    lhs =< rhs /\ ~ lhs == rhs.
-  Proof with discriminate || eauto.
-    cbn; intros [ | ] [ | ] H...
-    split...
-  Qed.
-
-  Lemma dir_compare_spec_EQ :
-    forall lhs : dir_t,
-    forall rhs : dir_t,
-    dir_compare lhs rhs = Eq ->
-    lhs == rhs.
-  Proof with discriminate || eauto.
-    cbn; intros [ | ] [ | ] H...
-  Qed.
-
-  Lemma dir_compare_spec_GT :
-    forall lhs : dir_t,
-    forall rhs : dir_t,
-    dir_compare lhs rhs = Gt ->
-    rhs =< lhs /\ ~ lhs == rhs.
-  Proof with discriminate || eauto.
-    cbn; intros [ | ] [ | ] H...
-    split...
-  Qed.
-
-  Lemma dir_list_compare_Eq :
-    forall lhs : list dir_t,
-    forall rhs : list dir_t,
-    lex_compare dir_compare lhs rhs = Eq <-> lhs = rhs.
-  Proof with discriminate || eauto.
-    induction lhs as [ | [ | ] lhs IH]; destruct rhs as [ | [ | ] rhs]; simpl; split; intros H_eq...
-    - apply eq_congruence, IH...
-    - apply IH; congruence.
-    - apply eq_congruence, IH...
-    - apply IH; congruence.
-  Qed.
-
   Definition index_t : Set :=
     list dir_t
   .
 
   Definition encoding_index (idx : index_t) : nat :=
-    fold_left (fun acc : nat => dir_t_rec (fun _ => nat) (2 * acc) (2 * acc + 1)) idx 1
+    fold_right (dir_t_rect (fun _ => nat -> nat) (fun acc : nat => 2 * acc) (fun acc : nat => 2 * acc + 1)) 1 idx
   .
 
-  Lemma encoding_index_last (idx : index_t) (d : dir_t) :
-    encoding_index (idx ++ [d]) =
-    match d with
-    | Dir_left => 2 * encoding_index idx
-    | Dir_right => 2 * encoding_index idx + 1
+  Lemma encoding_index_unfold (idx : index_t) :
+    encoding_index idx =
+    match idx with
+    | [] => 1
+    | Dir_left :: idx' => 2 * encoding_index idx'
+    | Dir_right :: idx' => 2 * encoding_index idx' + 1
     end.
-  Proof.
-    unfold encoding_index.
-    rewrite fold_left_last.
-    destruct d; reflexivity.
+  Proof with eauto.
+    induction idx as [ | [ | ] idx IH]; simpl...
   Qed.
 
   Lemma decoding_index :
@@ -124,8 +52,8 @@ Module BinTree.
       assert (claim6 : n / 2 <> 0)...
       destruct (acc_hyp (n / 2) claim4 claim5 claim6) as [idx H_idx].
       destruct (n mod 2) as [ | [ | n_mod_2]] eqn: H_obs...
-      { exists (idx ++ [Dir_left]); rewrite encoding_index_last... }
-      { exists (idx ++ [Dir_right]); rewrite encoding_index_last... }
+      { exists (Dir_left :: idx); rewrite encoding_index_unfold... }
+      { exists (Dir_right :: idx); rewrite encoding_index_unfold... }
   Qed.
 
   Lemma encoding_index_range :
@@ -133,8 +61,7 @@ Module BinTree.
     (exists idx : index_t, encoding_index idx = code) <-> code <> 0.
   Proof with lia || eauto.
     intros n; split.
-    - intros [idx H_idx]; subst n; pattern idx; revert idx; apply list_reversed_induction; cbn...
-      intros idx d H_ne; rewrite encoding_index_last; destruct d...
+    - intros [idx H_idx]; subst n; induction idx as [ | [ | ] idx IH]; simpl...
     - intros H_n_ne_0. destruct (decoding_index n H_n_ne_0) as [idx H_idx]...
   Qed.
 
@@ -146,16 +73,13 @@ Module BinTree.
   Proof with lia || eauto.
     assert (claim1 : forall idx : index_t, encoding_index idx > 0).
     { intros idx. enough (to_show : encoding_index idx <> 0)... pose (proj1 (encoding_index_range (encoding_index idx)))... }
-    intros idx1; pattern idx1; revert idx1; apply list_reversed_induction; cbn...
-    - intros idx2; pattern idx2; revert idx2; apply list_reversed_induction; cbn...
-      intros idx2 d2 _. pose (claim1 idx2). rewrite encoding_index_last; destruct d2...
-    - intros idx1 d1 IH.
-      intros idx2; pattern idx2; revert idx2; apply list_reversed_induction; cbn...
-      + pose (claim1 idx1). rewrite encoding_index_last. destruct d1...
-      + intros idx2 d2 _.
-        do 2 rewrite encoding_index_last; destruct d1; destruct d2...
-        { intros H_eq. apply (eq_congruence (fun idx : index_t => idx ++ [Dir_left]) idx1 idx2). apply IH... }
-        { intros H_eq. apply (eq_congruence (fun idx : index_t => idx ++ [Dir_right]) idx1 idx2). apply IH... }
+    induction idx1 as [ | d1 idx1 IH]; destruct idx2 as [ | d2 idx2]...
+    - pose (claim1 idx2); rewrite encoding_index_unfold; destruct d2; simpl...
+    - pose (claim1 idx1); rewrite encoding_index_unfold; destruct d1; simpl...
+    - rewrite encoding_index_unfold with (idx := d1 :: idx1).
+      rewrite encoding_index_unfold with (idx := d2 :: idx2).
+      destruct d1; destruct d2...
+      all: intros H_eq; apply eq_congruence, IH...
   Qed.
 
   End INDICES_OF_BINARY_TREES.
@@ -168,84 +92,28 @@ Module BinTree.
   Global Arguments BT_null {Elem}.
   Global Arguments BT_node {Elem}.
 
-  Definition bintreeExt_view {Elem : Type} : bintree Elem -> index_t -> option Elem :=
-    fix bintreeExt_view_fix (t : bintree Elem) (idx : index_t) {struct t} : option Elem :=
-    match t with
-    | BT_null => None
-    | BT_node t_l e t_r =>
-      match idx with
-      | [] => Some e
-      | Dir_left :: idx' => bintreeExt_view_fix t_l idx'
-      | Dir_right :: idx' => bintreeExt_view_fix t_r idx'
-      end
-    end
+  Definition btctx (Elem : Type) : Type :=
+    list (dir_t * (Elem * bintree Elem))
   .
-
-  Inductive btctx (Elem : Type) : Type :=
-  | Ctx_hole : btctx Elem
-  | Ctx_left (c_l : btctx Elem) (e : Elem) (t_r : bintree Elem) : btctx Elem
-  | Ctx_right (t_l : bintree Elem) (e : Elem) (c_r : btctx Elem) : btctx Elem
-  .
-
-  Global Arguments Ctx_hole {Elem}.
-  Global Arguments Ctx_left {Elem}.
-  Global Arguments Ctx_right {Elem}.
-
-  Definition combine_ctx {Elem : Type} : btctx Elem -> btctx Elem -> btctx Elem :=
-    fix combine_ctx_fix (c : btctx Elem) (c' : btctx Elem) : btctx Elem :=
-    match c with
-    | Ctx_hole => c'
-    | Ctx_left c_l e t_r => Ctx_left (combine_ctx_fix c_l c') e t_r
-    | Ctx_right t_l e c_r => Ctx_right t_l e (combine_ctx_fix c_r c')
-    end
-  .
-
-  Lemma combine_ctx_hole_l {Elem : Type} :
-    forall c1 : btctx Elem,
-    combine_ctx Ctx_hole c1 = c1.
-  Proof with eauto.
-    reflexivity.
-  Qed.
-
-  Lemma combine_ctx_hole_r {Elem : Type} :
-    forall c1 : btctx Elem,
-    combine_ctx c1 Ctx_hole = c1.
-  Proof with eauto.
-    induction c1 as [ | c_l IH e t_r | t_l e c_r IH]; simpl...
-    all: rewrite IH...
-  Qed.
-
-  Lemma combine_ctx_assoc {Elem : Type} :
-    forall c1 : btctx Elem,
-    forall c2 : btctx Elem,
-    forall c3 : btctx Elem,
-    combine_ctx c1 (combine_ctx c2 c3) = combine_ctx (combine_ctx c1 c2) c3.
-  Proof with eauto.
-    induction c1 as [ | c_l IH e t_r | t_l e c_r IH]; simpl...
-    - intros c2 c3.
-      enough (to_show : (combine_ctx c_l (combine_ctx c2 c3)) = (combine_ctx (combine_ctx c_l c2) c3))...
-      rewrite to_show...
-    - intros c2 c3.
-      enough (to_show : (combine_ctx c_r (combine_ctx c2 c3)) = (combine_ctx (combine_ctx c_r c2) c3))...
-      rewrite to_show...
-  Qed.
 
   Inductive btctx_spec {Elem : Type} (sub_t : bintree Elem) : btctx Elem -> bintree Elem -> Prop :=
-  | CtxSpec_hole
-    : btctx_spec sub_t (Ctx_hole) sub_t
+  | CtxSpec_top
+    : btctx_spec sub_t [] sub_t
   | CtxSpec_left c_l t_l e t_r
-    (H_btctx_spec_l : btctx_spec sub_t c_l t_l)
-    : btctx_spec sub_t (Ctx_left c_l e t_r) (BT_node t_l e t_r)
+    (H_l : btctx_spec sub_t c_l t_l)
+    : btctx_spec sub_t (c_l ++ [(Dir_left, (e, t_r))]) (BT_node t_l e t_r)
   | CtxSpec_right c_r t_l e t_r
-    (H_btctx_spec_r : btctx_spec sub_t c_r t_r)
-    : btctx_spec sub_t (Ctx_right t_l e c_r) (BT_node t_l e t_r)
+    (H_r : btctx_spec sub_t c_r t_r)
+    : btctx_spec sub_t (c_r ++ [(Dir_right, (e, t_l))]) (BT_node t_l e t_r)
   .
 
+  Local Hint Constructors btctx_spec : core.
+
   Lemma btctx_spec_refl {Elem : Type} (root : bintree Elem) :
-    btctx_spec root (Ctx_hole) root.
+    btctx_spec root [] root.
   Proof.
     constructor 1.
-  Defined.
+  Qed.
 
   Lemma btctx_spec_trans {Elem : Type} (root : bintree Elem) :
     forall t1 : bintree Elem,
@@ -254,39 +122,76 @@ Module BinTree.
     forall t2 : bintree Elem,
     forall c2 : btctx Elem,
     btctx_spec t2 c2 t1 ->
-    btctx_spec t2 (combine_ctx c1 c2) root.
+    btctx_spec t2 (c2 ++ c1) root.
   Proof.
     intros t1 c1 X1; induction X1; intros t2 c2 X2; simpl.
-    - exact X2.
-    - constructor 2; apply IHX1; exact X2.
-    - constructor 3; apply IHX1; exact X2.
-  Defined.
+    - rewrite app_nil_r; exact X2.
+    - rewrite app_assoc; constructor 2; apply IHX1; exact X2.
+    - rewrite app_assoc; constructor 3; apply IHX1; exact X2.
+  Qed.
 
-  Definition run_hole {Elem : Type} (sub_t : bintree Elem) : btctx Elem -> bintree Elem :=
-    fix run_hole_fix (c : btctx Elem) : bintree Elem :=
-    match c with
-    | Ctx_hole => sub_t
-    | Ctx_left c_l e t_r => BT_node (run_hole_fix c_l) e t_r
-    | Ctx_right t_l e c_r => BT_node t_l e (run_hole_fix c_r)
+  Definition recover_step_aux {Elem : Type} (d : dir_t) (e : Elem) (t : bintree Elem) : bintree Elem -> bintree Elem :=
+    match d with
+    | Dir_left => fun t_l : bintree Elem => BT_node t_l e t 
+    | Dir_right => fun t_r : bintree Elem => BT_node t e t_r
     end
   .
 
-  Lemma btctx_spec_run_hole {Elem : Type} :
-    forall root : bintree Elem,
-    forall c : btctx Elem,
-    forall sub_t : bintree Elem,
-    btctx_spec sub_t c root <-> run_hole sub_t c = root.
+  Definition recover_step {Elem : Type} : (dir_t * (Elem * bintree Elem)) -> bintree Elem -> bintree Elem :=
+    fun it : dir_t * (Elem * bintree Elem) =>
+    uncurry (recover_step_aux (fst it)) (snd it)
+  .
+
+  Definition recover {Elem : Type} (sub_t : bintree Elem) (c : btctx Elem) : bintree Elem :=
+    fold_right recover_step sub_t (rev c)
+  .
+
+  Lemma recover_unfold {Elem : Type} (sub_t : bintree Elem) c :
+    recover sub_t c =
+    match c with
+    | [] => sub_t
+    | (Dir_left, (e, t_r)) :: c' => recover (BT_node sub_t e t_r) c'
+    | (Dir_right, (e, t_l)) :: c' => recover (BT_node t_l e sub_t) c'
+    end.
+  Proof with eauto.
+    unfold recover at 1; rewrite fold_left_rev_right with (f := recover_step).
+    destruct c as [ | [[ | ] [e t]] c]; simpl...
+    all: unfold recover at 1; rewrite fold_left_rev_right with (f := recover_step)...
+  Qed.
+
+  Lemma recover_last {Elem : Type} (sub_t : bintree Elem) c d e t :
+    recover sub_t (c ++ [(d, (e, t))]) =
+    match d with
+    | Dir_left => BT_node (recover sub_t c) e t 
+    | Dir_right => BT_node t e (recover sub_t c)
+    end.
   Proof.
-    intros root c sub_t; split.
-    - intros X; induction X; simpl.
-      + reflexivity.
-      + rewrite IHX; reflexivity.
-      + rewrite IHX; reflexivity.
+    unfold recover at 1; rewrite list_rev_cons, fold_right_unfold; now destruct d.
+  Qed.
+
+  Theorem btctx_spec_recover {Elem : Type} sub_t c (root : bintree Elem) :
+    btctx_spec sub_t c root <-> recover sub_t c = root.
+  Proof with eauto.
+    split.
+    - intros X; induction X; simpl...
+      all: rewrite recover_last, IHX...
     - intros H_eq; subst root; revert sub_t.
-      induction c as [ | c_l IH e t_r | t_l e c_r IH]; simpl; intros sub_t.
-      + constructor 1.
-      + constructor 2; exact (IH sub_t).
-      + constructor 3; exact (IH sub_t).
+      pattern c; revert c; apply list_reversed_induction...
+      intros idx [[ | ] [e t]] IH sub_t; rewrite recover_last...
+  Qed.
+
+  Lemma btctx_spec_left {Elem : Type} c t_l e t_r (root : bintree Elem) :
+    btctx_spec (BT_node t_l e t_r) c root <-> btctx_spec t_l ((Dir_left, (e, t_r)) :: c) root.
+  Proof.
+    do 2 rewrite btctx_spec_recover.
+    now rewrite recover_unfold with (c := (Dir_left, (e, t_r)) :: c).
+  Qed.
+
+  Lemma btctx_spec_right {Elem : Type} c t_l e t_r (root : bintree Elem) :
+    btctx_spec (BT_node t_l e t_r) c root <-> btctx_spec t_r ((Dir_right, (e, t_l)) :: c) root.
+  Proof.
+    do 2 rewrite btctx_spec_recover.
+    now rewrite recover_unfold with (c := (Dir_right, (e, t_l)) :: c).
   Qed.
 
 End BinTree.
